feat: change Array.set to take a Nat and a tactic provided bound

src/Init/Data/Array/Set.lean
@@ -14,8 +14,8 @@ This will perform the update destructively provided that `a` has a reference
 count of 1 when called.
 -/
 @[extern "lean_array_fset"]
-def Array.set (a : Array α) (i : @& Fin a.size) (v : α) : Array α where
-  toList := a.toList.set i.val v
+def Array.set (a : Array α) (i : @& Nat) (v : α) (h : i < a.size := by get_elem_tactic): Array α where
+  toList := a.toList.set i v
 
 /--
 Set an element in an array, or do nothing if the index is out of bounds.
@@ -24,7 +24,7 @@ This will perform the update destructively provided that `a` has a reference
 count of 1 when called.
 -/
 @[inline] def Array.setD (a : Array α) (i : Nat) (v : α) : Array α :=
-  dite (LT.lt i a.size) (fun h => a.set ⟨i, h⟩ v) (fun _ => a)
+  dite (LT.lt i a.size) (fun h => a.set i v h) (fun _ => a)
 
 /--
 Set an element in an array, or panic if the index is out of bounds.
