src/Init/Meta.lean
@@ -443,7 +443,7 @@ def unsetTrailing (stx : Syntax) : Syntax :=
   if h : i < a.size then
     let v := a[i]
     match f v with
-    | some v => some <| a.set ⟨i, h⟩ v
+    | some v => some <| a.set i v h
     | none   => updateFirst a f (i+1)
   else
     none
